experiment/Experiment.Steel.Tac.fst
@@ -1,7 +1,10 @@
 module Experiment.Steel.Tac
 
-module L  = FStar.List.Pure
-module Fl = Learn.FList
+module L    = FStar.List.Pure
+module Fl   = Learn.FList
+module Vpl  = Experiment.Steel.VPropList
+module Msk  = Learn.List.Mask
+module Perm = Learn.Permutation
 
 open Learn.List.Mask
 open Steel.Effect
@@ -212,3 +215,246 @@ let rec check_map_to_eq_spec (#a : Type) (src trg : list a) (ij : Ll.vec (len sr
                          L.index trg (Some?.v (L.index ij i)) == L.index src i
                      with if i > 0
                           then assert (L.index ij i == L.index ij' (i-1) /\ L.index src i == L.index tl (i-1))
+
+
+(*** Building a [spec_find_ro] *)
+
+#push-options "--fuel 2"
+let rec ens_refl_impl_eqs
+      (#pre #post : Vpl.vprop_list) (#sl0 : Vpl.sl_f pre) (#sl1 : Vpl.sl_f post)
+      (#ens : Type0) (#es : list (sel_eq_t pre post))
+      (r : ens_refl sl0 sl1 ens es)
+      (e : sel_eq_t pre post)
+  : Lemma (requires  L.memP e es /\ ens) (ensures sl0 e._1 == U.cast _ (sl1 e._2))
+          (decreases r)
+  = match r with
+  | EnsEq e' p _ ->
+          assert (e == e')
+  | EnsConj #_ #_ #_ #_ #ens0 #ens1 #es0 #es1 r0 r1 ->
+          Ll.append_memP e es0 es1;
+          eliminate L.memP e es0 \/ L.memP e es1
+            returns sl0 e._1 == U.cast _ (sl1 e._2)
+               with _ . ens_refl_impl_eqs r0 e
+                and _ . ens_refl_impl_eqs (r1 ()) e
+#pop-options
+
+#push-options "--ifuel 0"
+let ograph_of_sl_eqs_spec
+      (#pre #post : Vpl.vprop_list)
+      (eqs : list (sel_eq_t pre post))
+      (i_post : Ll.dom post) (i_pre : Ll.dom pre)
+  : Lemma (L.index (L.index (ograph_of_sl_eqs eqs) i_post) i_pre <==>
+            (L.index pre i_pre == L.index post i_post /\ L.mem (i_pre, i_post) eqs))
+  =
+    let n_pre  = L.length pre  in
+    let n_post = L.length post in
+    let g0 = Ll.repeat n_post (Ll.repeat n_pre false) in
+    let f0 (i_pre : Ll.dom pre) (c : Ll.vec n_pre bool) : Ll.vec n_pre bool
+      = Ll.set i_pre true c     in
+    let f1 (g : ograph n_post n_pre) (e : sel_eq_t pre post) : ograph n_post n_pre
+      = let i_pre, i_post = e in Ll.map_nth i_post (f0 i_pre) g
+    in
+    assert (ograph_of_sl_eqs eqs == L.fold_left f1 g0 eqs) by (trefl ());
+    let p (eqs : list (sel_eq_t pre post)) (g : ograph n_post n_pre) : Type0 =
+      L.index (L.index g i_post) i_pre <==>
+         (L.index pre i_pre == L.index post i_post /\ L.mem (i_pre, i_post) eqs)
+    in
+    Ll.fold_left_ind f1 g0 eqs (fun eqs g _ -> p eqs g) (fun eqsl g e _ -> ());
+    assert (p (L.rev eqs) (ograph_of_sl_eqs eqs));
+    FStar.Classical.forall_intro (L.rev_mem eqs);
+    assert (p eqs (ograph_of_sl_eqs eqs))
+#pop-options
+
+#push-options "--fuel 0 --ifuel 0 --z3rlimit 20"
+let sel_eq_on_injection_iff_eq
+      (#pre #post : Vpl.vprop_list)
+      (f : Veq.partial_injection post pre)
+      (sl0 : Vpl.sl_f pre) (sl1 : Vpl.sl_f post)
+  : Lemma Vpl.(sel_eq_on (L.index f) sl0 sl1
+            <==> extract_vars (Veq.ij_matched_equiv f) (filter_sl (Msk.mask_not (Veq.ij_trg_mask f)) sl0)
+               == filter_sl (Msk.mask_not (Veq.ij_src_mask f)) sl1)
+  = Vpl.(
+    let m0 = Msk.mask_not (Veq.ij_trg_mask f) in
+    let m1 = Msk.mask_not (Veq.ij_src_mask f) in
+    let fsl0 = extract_vars (Veq.ij_matched_equiv f) (filter_sl m0 sl0) in
+    let fsl1 = filter_sl m1 sl1                                         in
+    introduce sel_eq_on (L.index f) sl0 sl1 ==> fsl0 == fsl1
+      with _ . Fl.flist_extensionality fsl0 fsl1
+      begin fun i1 ->
+        let i = Msk.mask_pull m1 i1 in
+        L.lemma_index_memP f i;
+        let Some j = L.index f i    in
+        let j1 = Msk.mask_push m0 j in
+        calc (==) {
+          (|_, fsl0 i1|) <: t : Type & t;
+        == { }
+          (|_, filter_sl m0 sl0 (Veq.ij_matched_equiv f i1)|);
+        == { }
+          (|_, filter_sl m0 sl0 j1|);
+        == { }
+          (|_, sl0 j|);
+        == {(*by assumption*)}
+          (|_, sl1 i|);
+        == { }
+          (|_, fsl1 i1|);
+        }
+      end;
+    introduce fsl0 == fsl1 ==> sel_eq_on (L.index f) sl0 sl1
+      with _ . introduce forall (i : Ll.dom post {Some? (L.index f i)}) .
+                         sl0 (Some?.v (L.index f i)) == U.cast _ (sl1 i)
+      with begin
+        L.lemma_index_memP f i;
+        let Some j = L.index f i    in
+        let i1 = Msk.mask_push m1 i in
+        let j1 = Msk.mask_push m0 j in
+        calc (==) {
+          (|_, sl1 i|) <: t : Type & t;
+        == { }
+          (|_, fsl1 i1|);
+        == {(*by assumption*)}
+          (|_, fsl0 i1|);
+        == { }
+          (|_, filter_sl m0 sl0 (Veq.ij_matched_equiv f i1)|);
+        == { }
+          (|_, filter_sl m0 sl0 j1|);
+        == { }
+          (|_, sl0 j|);
+        }
+      end
+  )
+#pop-options
+
+// TODO:MOVE
+#push-options "--fuel 0 --ifuel 0"
+let pequiv_trans_sym #a (#l0 #l1 #l2 : list a) (f : Perm.pequiv l0 l1) ($g : Perm.pequiv l1 l2)
+  : Lemma Perm.(pequiv_sym (pequiv_trans f g) == pequiv_trans (pequiv_sym g) (pequiv_sym f))
+  =
+    let rew1 () : Lemma (L.length l1 == L.length l0) = () in
+    let rew2 () : Lemma (L.length l2 == L.length l0) = () in
+    assert Perm.(eq2 #(perm_f (L.length l2))
+                      (pequiv_sym (pequiv_trans f g)) (pequiv_trans (pequiv_sym g) (pequiv_sym f)))
+      by (norm [delta_only [`%Perm.pequiv_sym; `%Perm.pequiv_trans; `%U.cast]; iota];
+          l_to_r [(`(`@rew1)); (`(`@rew2))];
+          with_policy Goal (fun () -> apply_lemma (`Perm.inv_f_comp));
+          l_to_r [(`(`@rew1)); (`(`@rew2))])
+
+let pequiv_append_sym #a (#l0 #l0' : list a) ($f0 : Perm.pequiv l0 l0')
+                         (#l1 #l1' : list a) ($f1 : Perm.pequiv l1 l1')
+  : Lemma Perm.(pequiv_sym (pequiv_append f0 f1) == pequiv_append (pequiv_sym f0) (pequiv_sym f1))
+  =
+    let rew0 () : Lemma L.(length l0' == length l0) = () in
+    let rew1 () : Lemma L.(length l1' == length l1) = () in
+    let rew2 () : Lemma L.(eq2 #nat (length (l0' @ l1')) (length l0 + length l1)) = () in
+    let rew3 () : Lemma L.(eq2 #nat (length (l0  @ l1 )) (length l0 + length l1)) = () in
+    assert Perm.(eq2 #(perm_f L.(length (l0' @ l1')))
+                      (pequiv_sym (pequiv_append f0 f1)) (pequiv_append (pequiv_sym f0) (pequiv_sym f1)))
+      by (norm [delta_only [`%Perm.pequiv_sym; `%Perm.pequiv_append; `%U.cast]; iota];
+          l_to_r [(`(`@rew0)); (`(`@rew1)); (`(`@rew2)); (`(`@rew3))];
+          apply_lemma (`Perm.perm_f_append_inv))
+
+let pequiv_sym_sym #a (#l0 #l1 : list a) ($f : Perm.pequiv l0 l1)
+  : Lemma Perm.(pequiv_sym (pequiv_sym f) == f)
+  =
+    let rew () : Lemma L.(length l1 == length l0) = () in
+    assert Perm.(eq2 #(perm_f (L.length l0)) (pequiv_sym (pequiv_sym f)) f)
+      by (norm [delta_only [`%Perm.pequiv_sym; `%U.cast]; iota];
+          l_to_r [``@rew];
+          apply_lemma (`Perm.inv_f_invol))
+
+let extract_vars_index
+      (#src #dst : Vpl.vprop_list) (p : Vpl.vequiv_perm src dst)
+      (xs : Vpl.sl_f src) (i : Ll.dom dst)
+  : Lemma (Vpl.extract_vars p xs i === xs (p i))
+  = ()
+
+let if_eq_else #a guard (thn els : a)
+  : Lemma (requires not guard) (ensures (if guard then thn else els) == els)
+  = ()
+
+let append_vars_index_right (#v0 #v1 : Vpl.vprop_list) (sl0 : Vpl.sl_f v0) (sl1 : Vpl.sl_f v1)
+                            (i : Fin.fin L.(length v1))
+  : Lemma (Vpl.append_vars sl0 sl1 (L.length v0 + i) === sl1 i)
+  = Ll.pat_append ()
+
+#push-options "--z3rlimit 20"
+let build_spec_find_ro_from_ij_lem1
+      (pre post : Vpl.vprop_list) (ij : Veq.partial_injection post pre)
+      (p0 : Vpl.vequiv_perm (Msk.filter_mask (Msk.mask_not (Veq.ij_trg_mask ij)) pre)
+                            (Msk.filter_mask (Msk.mask_not (Veq.ij_src_mask ij)) post))
+      (sl1    : Vpl.sl_f Msk.(filter_mask (Veq.ij_src_mask ij) post))
+      (sl_fr1 : Vpl.sl_f Msk.(filter_mask (mask_not (Veq.ij_trg_mask ij)) pre))
+  : Lemma Vpl.(extract_vars p0 sl_fr1
+            == filter_sl (Msk.mask_not (Veq.ij_src_mask ij))
+                  (extract_vars Perm.(pequiv_sym (pequiv_trans
+                    (Msk.mask_pequiv_append (Veq.ij_src_mask ij) post)
+                    (pequiv_append (pequiv_refl _) (pequiv_sym p0)))
+                  ) (append_vars sl1 sl_fr1)))
+  = Vpl.(
+    let m0    = Msk.mask_not (Veq.ij_trg_mask ij) in
+    let m1    = Msk.mask_not (Veq.ij_src_mask ij) in
+    let m1'   = Veq.ij_src_mask ij                in
+    let n1'   = Msk.mask_len m1'                  in
+    let ro    = Msk.filter_mask m0  pre           in
+    let ro'   = Msk.filter_mask m1  post          in
+    let post' = Msk.filter_mask m1' post          in
+
+    let p0   : vequiv_perm ro ro' = p0                                  in
+    let p1a  = Msk.mask_pequiv_append m1' post                          in
+    let p1b  = Perm.(pequiv_append (pequiv_refl post') (pequiv_sym p0)) in
+    let p1   : Vpl.vequiv_perm post L.(post' @ ro)
+             = Perm.(pequiv_trans p1a p1b)                              in
+    let p1'a = Msk.mask_pequiv_append' m1' post                         in
+    let p1'b = Perm.(pequiv_append (pequiv_refl post') p0)              in
+    let p1' : Vpl.vequiv_perm L.(post' @ ro) post
+            = Perm.(pequiv_trans p1'b p1'a)                             in
+
+    U.assert_by (Perm.pequiv_sym p1 == p1') Perm.(fun () ->
+      pequiv_trans_sym p1a p1b;
+      pequiv_append_sym (pequiv_refl post') (pequiv_sym p0);
+      Msk.mask_perm_append_inv m1'
+    );
+
+    let sl1'a = append_vars sl1 sl_fr1 in
+    let sl1'  = extract_vars p1' sl1'a in
+    Fl.flist_extensionality (extract_vars p0 sl_fr1) (filter_sl m1 sl1') (fun i1 ->
+      let i0 = Msk.mask_pull m1 i1 in
+      let i2 = n1' + i1            in
+      let j1 = p0 i1               in
+      assert (L.length post' == n1');
+      calc (==) {
+        (|_, filter_sl m1 sl1' i1|) <: t : Type & t;
+      == { }
+        (|_, sl1' i0|);
+      == { }
+        (|_, extract_vars p1' sl1'a i0|);
+      == { extract_vars_index p1' sl1'a i0 }
+        (|_, sl1'a (p1' i0)|);
+      == { assert (p1' i0 == p1'b (p1'a i0));
+           Msk.mask_perm_append'_index m1' i0;
+           assert (p1'a i0 == i2) }
+        (|_, sl1'a (p1'b i2)|);
+      == { let rew () : Lemma (L.length (Msk.filter_mask m1' post) == n1') = () in
+           assert (p1'b i2 == n1' + p0 i1)
+             by (norm [delta_only [`%Perm.pequiv_append; `%Perm.perm_f_append; `%Perm.mk_perm_f;
+                                   `%U.cast; `%FunctionalExtensionality.on];
+                       iota];
+                 l_to_r [``@rew];
+                 clear_all ();
+                 apply_lemma (`U.eq2_trans);
+                   apply_lemma (`if_eq_else); smt ();
+                 smt ()) }
+        (|_, sl1'a (n1' + j1)|);
+      == { }
+        (|_, append_vars sl1 sl_fr1 (n1' + j1)|);
+      == { append_vars_index_right sl1 sl_fr1 j1 }
+        (|_, sl_fr1 j1|);
+      == { extract_vars_index p0 sl_fr1 i1 }
+        (|_, extract_vars p0 sl_fr1 i1|);
+      }
+    )
+  )
+#pop-options
+
+#pop-options
+
+(**) private let __end_build_spec_find_ro_from_ij = ()
