experiment/Experiment.Steel.fsti
@@ -127,10 +127,6 @@ let prog_LV_to_Fun_extract_wp
 
 (**** normalisation steps *)
 
-let __delta_list : list string =
-  [`%L.length; `%L.index; `%L.op_At; `%L.append; `%L.map; `%L.hd; `%L.tl; `%L.tail; `%L.count;
-   `%Ll.initi; `%Ll.repeat]
-
 let __normal_M : list norm_step = [
   delta_only [`%Vpl.vprop_list_sels_t;   `%M.Mkrepr?.repr_tree;
               `%L.map; `%SE.Mkvprop'?.t];
@@ -141,7 +137,7 @@ let __normal_M : list norm_step = [
 ]
 
 let __normal_lc_sub_push : list norm_step = [
-  delta_only (L.append __delta_list
+  delta_only (L.append TcS.__delta_list
              [`%LV.lc_sub_push; `%LV.lc_sub_push_aux;
               `%Perm.perm_f_to_list; `%Perm.perm_f_of_list;
               `%Perm.comp; `%Perm.mk_perm_f; `%Perm.perm_f_append; `%Perm.perm_f_cons; `%Perm.id_n;
@@ -152,10 +148,10 @@ let __normal_lc_sub_push : list norm_step = [
 ]
 
 let __normal_LV2SF : list norm_step = [
-  delta_only (L.append __delta_list
+  delta_only (L.append TcS.__delta_list
              [`%prog_LV_to_Fun; `%LV2SF.repr_SF_of_LV;
-              `%Vpl.vprop_list_sels_t;
-              `%LV.sub_prd_sl; `%LV.eij_sl; `%LV.filter_sl; `%LV.res_sel;
+              `%Vpl.vprop_list_sels_t; `%Vpl.filter_sl;
+              `%LV.sub_prd_sl; `%LV.eij_sl; `%LV.res_sel;
               `%M.post_sl_t;
               `%Fl.dlist_of_f; `%Fl.apply_perm_r; `%Fl.append; `%Fl.splitAt_ty;
               `%Dl.initi;
